

Week 11: Integration by Parts

Lecturer: Zhi (George) Lin

Calculus 1, Class 6

Nov 12th 2025

Summary

- 1 Quiz Reminder
- 2 Total Derivative
- 3 Integration by Parts (IBP)
- 4 Repeated IBP
- 5 Cyclic IBP
- 6 Classics via IBP
- 7 Laplace-type Integrals
- 8 Gamma Function
- 9 Conclusion

Quiz Reminder

Time: 11/19 (Wed) 17:30-18:20
Quiz Scope: 5.1 - 6.1
Location: 普通103
TA Hour: Fri. 14-16
化學系館（積學館）B363

Today's Goals

By the end, you should be able to:

- Recognize when to use IBP vs. substitution/other methods.
- Apply one-shot IBP, repeated/tabular IBP, and cyclic IBP (solve for I).
- Derive and use classic identities obtained via IBP.
- Avoid common pitfalls (bad u , sign errors, boundary terms).

Total derivative viewpoint: why “ $\times dx$ ” is OK

Total derivative (1D). For differentiable $f : \mathbb{R} \rightarrow \mathbb{R}$,

$$Df(x)[h] = f'(x) h \quad \Rightarrow \quad df := Df(x)[dx] = f'(x) dx.$$

Leibniz rule. $D(uv) = u Dv + v Du$. Evaluating at dx gives

$$\boxed{d(uv) = u dv + v du} \quad \Rightarrow \quad u dv = d(uv) - v du.$$

Interpret “ $\times dx$ ” as: *evaluate the linear map at the increment dx* , not as cancelling a denominator.

Understanding $Df(x)[h] = f'(x) h$

Total derivative: $Df(x)$ is the linear map that gives the change in f for a small input change h :

$$Df(x)[h] = f'(x) h.$$

In words: “if x changes by h , f changes by about $f'(x) h$.”

Setting the input change to the infinitesimal dx gives the differential form:

$$df := Df(x)[dx] = f'(x) dx.$$

Thus “ $\times dx$ ” means we *apply the total derivative to the increment dx* , not that we cancel a denominator.

When “ $\times dx$ ” is legitimate (\checkmark)

- **Convert derivatives to differentials (same variable):**

$$\frac{d}{dx}(uv) = u v' + v u' \iff d(uv) = u dv + v du.$$

- **Chain rule (substitution):**

$$\frac{d}{dx}F(g(x)) = F'(g)g' \iff dF = F'(g) dg, dg = g'(x) dx.$$

- **Separation of variables (ODE):** If $\frac{dy}{dx} = F(x)G(y)$, then

$$\frac{1}{G(y)} dy = F(x) dx \text{ (then integrate).}$$

- **Multivariable total differential:** $df = f_x dx + f_y dy$; along $y = y(x)$,
 $dy = y'(x) dx$.

When not to “ $\times dx$ ” (\times)

1. Not a fraction — $\frac{d}{dx}$ is an operator.

- You can multiply by dx *after* differentiation, not before.
- Wrong: $(d/dx)(fg) dx = df \cdot dg$ (this skips the product rule).
Correct: $d(fg) = f dg + g df$.

2. Don't ignore other variables.

- In several variables, $df = f_x dx + f_y dy + \dots$.
- Writing $df = f_x dx$ is only valid if $dy = dz = \dots = 0$ (holding others fixed).
- Example: $f(x, y) = xy \Rightarrow df = y dx + x dy$.

IBP: Derivation and The Rule

From the product rule,

$$\frac{d}{dx}(uv) = u v' + v u' \implies u dv = d(uv) - v du.$$

Integrating both sides,

$$\boxed{\int u dv = uv - \int v du}.$$

Choice of u and dv : pick u so that du simplifies; pick dv so that v is easy to find.

Choosing u : Heuristics and When *Not* to Use IBP

Heuristics (LIATE/ILATE): Logarithmic \rightarrow Inverse trig \rightarrow Algebraic \rightarrow Trig \rightarrow Exponential.

- Use as a *tiebreaker*, not a law. Ask: does differentiating u *simplify*? does integrating dv stay easy?

Often better than IBP:

- Pure rational functions \Rightarrow partial fractions.
- Obvious chain rule \Rightarrow substitution.
- Trig powers \Rightarrow trig identities first.

Cyclic case: for $\int e^x \sin x \, dx$ or $\int e^x \cos x \, dx$, use IBP twice and solve for I .

Compute using one-shot IBP:

$$\int x e^x dx = e^x(x - 1) + C,$$

$$\int x \sin x dx = -x \cos x + \sin x + C,$$

$$\int \ln x dx = x \ln x - x + C,$$

$$\int \arctan x dx = x \arctan x - \frac{1}{2} \ln(1 + x^2) + C.$$

Emphasize the choice $u = \ln x, \arctan x$ (they simplify upon differentiation).

Repeated (Tabular) IBP: When and How

When: polynomial \times (exp or sin/cos) — the polynomial “dies” under differentiation.

D–I table idea:

Differentiate	Integrate
x^n	$e^{ax}, \sin bx, \cos bx$

Alternate signs; stop when the derivative hits 0.

Example (Tabular): $\int x^3 e^x dx$

$$\int x^3 e^x dx = e^x (x^3 - 3x^2 + 6x - 6) + C.$$

(Derivative chain of x^3 : $x^3, 3x^2, 6x, 6, 0$; integrate e^x repeatedly; alternate signs.)

Cyclic IBP: Solve for the Integral

Let $I = \int e^x \cos x \, dx$. One IBP gives an integral with $\sin x$; doing IBP again returns to I . Collect terms:

$$2I = e^x (\sin x + \cos x) \quad \Rightarrow \quad \boxed{I = \frac{e^x}{2} (\sin x + \cos x) + C}.$$

Same idea works for $\int e^x \sin x \, dx$.

Cyclic IBP: Detailed Solution for $\int e^x \cos x \, dx$

Let

$$I = \int e^x \cos x \, dx.$$

First IBP. Choose $u = e^x$, $dv = \cos x \, dx$. Then $du = e^x \, dx$, $v = \sin x$. Hence

$$I = \int u \, dv = uv - \int v \, du = e^x \sin x - \int e^x \sin x \, dx.$$

Set

$$J = \int e^x \sin x \, dx,$$

so the first step gives $I = e^x \sin x - J$.

Second IBP (for J). Again take $u = e^x$, $dv = \sin x \, dx$. Then $du = e^x \, dx$, $v = -\cos x$. Thus

$$J = \int u \, dv = uv - \int v \, du = -e^x \cos x + \int e^x \cos x \, dx = -e^x \cos x + I.$$

Cyclic IBP: Detailed Solution for $\int e^x \cos x \, dx$

Close the cycle and solve for I .

$$I = e^x \sin x - J = e^x \sin x - (-e^x \cos x + I) = e^x(\sin x + \cos x) - I.$$

Therefore

$$2I = e^x(\sin x + \cos x) \quad \Longrightarrow \quad \boxed{I = \frac{e^x}{2}(\sin x + \cos x) + C}.$$

(A) Logarithm:

$$\int \ln x \, dx = x \ln x - x + C.$$

(B) Inverse tangent:

$$\int \arctan x \, dx = x \arctan x - \frac{1}{2} \ln(1 + x^2) + C.$$

(C) General log moment:

$$\boxed{\int x^n \ln x \, dx = \frac{x^{n+1}}{n+1} \left(\ln x - \frac{1}{n+1} \right) + C}.$$

Derivation: $\int x^n \ln x \, dx$ (for $n \neq -1$, $x > 0$)

Use integration by parts with

$$u = \ln x \quad \Rightarrow \quad du = \frac{1}{x} dx, \quad dv = x^n dx \quad \Rightarrow \quad v = \frac{x^{n+1}}{n+1} \quad (n \neq -1).$$

Then

$$\int x^n \ln x \, dx = uv - \int v \, du = \frac{x^{n+1}}{n+1} \ln x - \int \frac{x^{n+1}}{n+1} \cdot \frac{1}{x} dx.$$

Simplify the remaining integral:

$$\int \frac{x^{n+1}}{n+1} \cdot \frac{1}{x} dx = \frac{1}{n+1} \int x^n dx = \frac{1}{n+1} \cdot \frac{x^{n+1}}{n+1}.$$

Therefore,

$$\int x^n \ln x \, dx = \frac{x^{n+1}}{n+1} \ln x - \frac{x^{n+1}}{(n+1)^2} + C = \boxed{\frac{x^{n+1}}{n+1} \left(\ln x - \frac{1}{n+1} \right) + C}.$$

Special case $n = -1$: $\int \frac{\ln x}{x} dx = \frac{1}{2}(\ln x)^2 + C.$

Exponential-Trig (Laplace-type) Integrals ($a > 0$)

Two IBPs (or integrate $e^{-ax} \cos bx$ directly) yield

$$\boxed{\int_0^{\infty} e^{-ax} \cos(bx) dx = \frac{a}{a^2 + b^2}, \quad \int_0^{\infty} e^{-ax} \sin(bx) dx = \frac{b}{a^2 + b^2}}.$$

Always justify boundary terms: $e^{-ax} \cos(bx) \rightarrow 0$ as $x \rightarrow \infty$ when $a > 0$.

Derivation by Cyclic IBP ($a > 0$)

Define

$$C := \int_0^\infty e^{-ax} \cos(bx) dx, \quad S := \int_0^\infty e^{-ax} \sin(bx) dx, \quad (a > 0, b \in \mathbb{R}).$$

Step 1: IBP for C . Let $u = e^{-ax}$, $dv = \cos(bx) dx$. Then $du = -ae^{-ax} dx$, $v = \frac{1}{b} \sin(bx)$.

$$C = \left[e^{-ax} \cdot \frac{1}{b} \sin(bx) \right]_0^\infty - \int_0^\infty \frac{1}{b} \sin(bx) (-ae^{-ax}) dx = \frac{a}{b} S.$$

(Boundary term vanishes since $e^{-ax} \rightarrow 0$ as $x \rightarrow \infty$ and $\sin(0) = 0$.)

Derivation by Cyclic IBP ($a > 0$)

Step 2: IBP for S . Let $u = e^{-ax}$, $dv = \sin(bx) dx$. Then $du = -ae^{-ax} dx$, $v = -\frac{1}{b} \cos(bx)$.

$$\begin{aligned} S &= \left[e^{-ax} \cdot \left(-\frac{1}{b} \cos(bx) \right) \right]_0^\infty - \int_0^\infty \left(-\frac{1}{b} \cos(bx) \right) (-ae^{-ax}) dx \\ &= \frac{1}{b} - \frac{a}{b} C. \end{aligned}$$

(Boundary term: at ∞ it is 0; at 0 it is $-\frac{1}{b} \cos 0 = -\frac{1}{b}$; subtracting yields $+\frac{1}{b}$.)

Derivation by Cyclic IBP ($a > 0$)

Step 3: Solve the linear system. From Step 1, $C = \frac{a}{b}S$. Substitute into Step 2:

$$S = \frac{1}{b} - \frac{a}{b} \cdot \frac{a}{b}S \implies S\left(1 + \frac{a^2}{b^2}\right) = \frac{1}{b} \implies \boxed{S = \frac{b}{a^2 + b^2}}.$$

Then

$$\boxed{C = \frac{a}{b}S = \frac{a}{a^2 + b^2}}.$$

Checks. If $b = 0$: $C = \int_0^\infty e^{-ax} dx = \frac{1}{a}$ and $S = 0$. The formulas give $\frac{a}{a^2+0} = \frac{1}{a}$ and $\frac{0}{a^2+0} = 0$, consistent.

Boundary justification: For $a > 0$, e^{-ax} dominates any bounded trig factor, so $e^{-ax} \cos(bx) \rightarrow 0$, $e^{-ax} \sin(bx) \rightarrow 0$ as $x \rightarrow \infty$.

Gamma Function: Explicit Definition

Definition (Euler integral of the second kind). For $\Re(s) > 0$,

$$\Gamma(s) := \int_0^{\infty} x^{s-1} e^{-x} dx$$

This integral converges because x^{s-1} is integrable near 0 when $\Re(s) > 0$, and e^{-x} decays exponentially as $x \rightarrow \infty$.

Basic values.

$$\Gamma(1) = \int_0^{\infty} e^{-x} dx = 1, \quad \Gamma\left(\frac{1}{2}\right) = \int_0^{\infty} x^{-1/2} e^{-x} dx = \sqrt{\pi}.$$

Connection to Factorials and Your I_n

For $n \in \mathbb{N} \cup \{0\}$, set $I_n = \int_0^\infty x^n e^{-x} dx$ (from the previous slide). Then with $s = n + 1$,

$$I_n = \int_0^\infty x^{(n+1)-1} e^{-x} dx = \Gamma(n+1).$$

IBP recursion: For $n \geq 1$,

$$I_n = n I_{n-1} \quad \Longleftrightarrow \quad \Gamma(n+1) = n \Gamma(n).$$

Since $\Gamma(1) = 1$, induction yields the **factorial identity**

$$\boxed{\Gamma(n+1) = n! \quad (n = 0, 1, 2, \dots)}.$$

(Optional) Extension Beyond Integers

For $s > 0$ define $\Gamma(s) = \int_0^\infty x^{s-1} e^{-x} dx$. The same IBP yields the functional equation

$$\Gamma(s+1) = s\Gamma(s), \quad \Gamma(1) = 1.$$

Thus $\Gamma(n+1) = n!$ for integers $n \geq 0$, and Γ extends the factorial to nonintegers (e.g. $\Gamma(\frac{1}{2}) = \sqrt{\pi}$).

(Optional) Quick Table of Explicit Values

$$\Gamma(1) = 1, \quad \Gamma(2) = 1!, \quad \Gamma(3) = 2!, \quad \Gamma(4) = 3!, \quad \dots$$

$$\Gamma\left(\frac{1}{2}\right) = \sqrt{\pi}, \quad \Gamma\left(\frac{3}{2}\right) = \frac{1}{2}\sqrt{\pi}, \quad \Gamma\left(\frac{5}{2}\right) = \frac{3}{4}\sqrt{\pi}, \quad \Gamma\left(\frac{7}{2}\right) = \frac{15}{8}\sqrt{\pi}.$$

Pattern for half-integers: for $k \in \mathbb{N}$,

$$\Gamma\left(k + \frac{1}{2}\right) = \frac{(2k-1)!!}{2^k} \sqrt{\pi} = \frac{(2k)!}{4^k k!} \sqrt{\pi}.$$

Common Pitfalls

- Choosing u that *does not* simplify upon differentiation.
- Forgetting the minus: $\int u dv = uv - \int v du$.
- Swapping u and dv mid-calculation.
- In cyclic IBP, forgetting to collect terms and solve for the original I .

Identity Toolbox (Handy Results)

- $\int \ln x \, dx = x \ln x - x + C$
- $\int \arctan x \, dx = x \arctan x - \frac{1}{2} \ln(1 + x^2) + C$
- $\int x^n \ln x \, dx = \frac{x^{n+1}}{n+1} \left(\ln x - \frac{1}{n+1} \right) + C$
- $\int_0^1 x^m \ln x \, dx = -\frac{1}{(m+1)^2} \quad (m > -1)$
- $I_n = \int_0^{\pi/2} \sin^n x \, dx = \frac{n-1}{n} I_{n-2}$
- $\int_0^\infty e^{-ax} \cos(bx) \, dx = \frac{a}{a^2 + b^2}, \quad \int_0^\infty e^{-ax} \sin(bx) \, dx = \frac{b}{a^2 + b^2} \quad (a > 0)$
- $\int_0^\infty x^n e^{-x} \, dx = n! \quad (\text{Gamma at integers})$